moving tries to separate theory; more

Weidenbach_Book/CDCL_Two_Watched_Literals_List_Simple_Code.thy
@@ -9,9 +9,6 @@ definition backtrack_l' :: "'v twl_st_l \<Rightarrow> 'v twl_st_l nres" where
       do {
         ASSERT(M \<noteq> []);
         let L = lit_of (hd M);
-        ASSERT(get_level M L = count_decided M);
-        ASSERT(\<exists>K M1 M2. (Decided K # M1, M2) \<in> set (get_all_ann_decomposition M) \<and>
-          get_level M K = get_maximum_level M (mset (the D) - {#-L#}) + 1);
         let j = snd (the (find_level_decomp M (the D) [] (count_decided M)));
         let M1 = tl (the (bt_cut j M));
 
@@ -63,11 +60,9 @@ proof-
     apply (refine_rcg; remove_dummy_vars)
     subgoal by simp
     subgoal by simp
-    subgoal by simp
-    subgoal by simp
     subgoal premises p for M N U C NP UP WS Q L
     proof -
-      note S = p(1) and L = p(4) and M_not_empty = p(2) and ex_decomp = p(8)
+      note S = p(1) and L = p(4) and M_not_empty = p(2) and L_hd = p(4) and ex_decomp = p(6)
       have n_d: \<open>no_dup M\<close>
         using struct_invs unfolding twl_struct_invs_def cdcl\<^sub>W_restart_mset.cdcl\<^sub>W_all_struct_inv_def cdcl\<^sub>W_restart_mset.cdcl\<^sub>W_M_level_inv_def
         by (simp add: cdcl\<^sub>W_restart_mset_state S)
@@ -83,7 +78,7 @@ proof-
       obtain M1'' M2'' K'' where
         decomp_K'': \<open>(Decided K'' # M1'', M2'') \<in> set (get_all_ann_decomposition M)\<close>
         \<open>get_level M K'' = Suc (get_maximum_level M (remove1_mset (- lit_of (hd M)) (mset C')))\<close>
-        using ex_decomp by auto
+        using ex_decomp L_hd by auto
       then have lev_max: \<open>get_maximum_level M (mset (remove1 (-L) C')) < count_decided M\<close>
         using count_decided_ge_get_level[of M K''] L by auto
       have \<open>-L \<in># mset C'\<close>
@@ -119,7 +114,7 @@ proof-
     qed
     subgoal premises p for M N U C NP UP WS Q L M1
     proof -
-      note S = p(1) and L_hd = p(4) and len_C = p(11)
+      note S = p(1) and L_hd = p(4) and len_C = p(9)
       obtain C' where [simp]: \<open>C = Some C'\<close>
         using confl1 S by auto
 
@@ -358,310 +353,16 @@ lemma cdcl_twl_stgy_prog_l'_spec_final:
   using assms by (auto simp: full_def pending_l_pending get_conflict_l_get_conflict
       pw_conc_inres pw_conc_nofail pw_ords_iff(1))
 
-
-schematic_goal valued_impl: "RETURN ?c \<le> valued M L"
-  unfolding unit_propagation_inner_loop_body_l_def valued_def Let_def
+schematic_goal backtrack_l'_impl: "RETURN ?c \<le> backtrack_l' S"
+  unfolding backtrack_l'_def valued_def Let_def
   apply (refine_transfer find_unwatched_impl)
   done
 
-concrete_definition valued_impl uses valued_impl
+concrete_definition backtrack_l'_impl uses backtrack_l'_impl
 
-prepare_code_thms valued_impl_def
-export_code valued_impl in SML
-
-declare find_unwatched_impl[refine_transfer] valued_impl[refine_transfer]
-schematic_goal unit_propagation_inner_loop_body_list: "RETURN ?c \<le> unit_propagation_inner_loop_body_l L C S"
-  unfolding unit_propagation_inner_loop_body_l_def
-  apply (refine_transfer)
-  done
-
-(*
-To generate code, remove assertions!
-concrete_definition backtrack_l''_impl uses
-  backtrack_l'_def
-prepare_code_thms backtrack_l''_impl_def
-thm backtrack_l''_impl_def
-export_code backtrack_l''_impl in Haskell *)
-term nat_assn
-abbreviation \<open>nat_ann_lit_assn \<equiv> (id_assn :: (nat, nat) ann_lit \<Rightarrow> _)\<close>
-abbreviation \<open>nat_lit_assn \<equiv> (id_assn :: nat literal \<Rightarrow> _)\<close>
-
-
-instance literal :: (heap) heap
-proof standard
-  obtain f :: \<open>'a \<Rightarrow> nat\<close> where f: \<open>inj f\<close>
-    by blast
-  then have Hf: \<open>f x = f s \<longleftrightarrow> x = s\<close> for s x
-    unfolding inj_on_def Ball_def comp_def by blast
-  let ?f = \<open>\<lambda>L. (is_pos L, f (atm_of L))\<close>
-  have \<open>OFCLASS(bool \<times> nat, heap_class)\<close>
-   by standard
-  then obtain g :: \<open>bool \<times> nat \<Rightarrow> nat\<close> where g: \<open>inj g\<close>
-    by blast
-  then have H: \<open>g (x, y) = g (s, t) \<longleftrightarrow> x = s \<and> y = t\<close> for s t x y
-    unfolding inj_on_def Ball_def comp_def by blast
-  have \<open>inj (g o ?f)\<close>
-    using f g unfolding inj_on_def Ball_def comp_def H Hf
-    apply (intro allI impI)
-    apply (rename_tac x y, case_tac x; case_tac y)
-    by auto
-  then show \<open>\<exists>to_nat:: 'a literal \<Rightarrow> nat. inj to_nat\<close>
-    by blast
-qed
-
-instance ann_lit :: (heap, heap) heap
-proof standard
-  let ?f = \<open>\<lambda>L:: ('a, 'b) ann_lit. (lit_of L, if is_decided L then None else Some (mark_of L))\<close>
-  have f: \<open>inj ?f\<close>
-    unfolding inj_on_def Ball_def
-    apply (intro allI impI)
-    apply (rename_tac x y, case_tac x; case_tac y)
-    by auto
-  then have Hf: \<open>?f x = ?f s \<longleftrightarrow> x = s\<close> for s x
-    unfolding inj_on_def Ball_def comp_def by blast
-  have \<open>OFCLASS('a literal \<times> 'b option, heap_class)\<close>
-   by standard
-  then obtain g :: \<open>'a literal \<times> 'b option \<Rightarrow> nat\<close> where g: \<open>inj g\<close>
-    by blast
-  then have H: \<open>g (x, y) = g (s, t) \<longleftrightarrow> x = s \<and> y = t\<close> for s t x y
-    unfolding inj_on_def Ball_def comp_def by blast
-  have \<open>inj (g o ?f)\<close>
-    using f g unfolding inj_on_def Ball_def comp_def H Hf
-    apply (intro allI impI)
-    apply (rename_tac x y, case_tac x; case_tac y)
-    by auto
-  then show \<open>\<exists>to_nat:: ('a, 'b) ann_lit \<Rightarrow> nat. inj to_nat\<close>
-    by blast
-qed
-
-term valued
-term nfoldli
-
-definition valued'  :: "('a, 'b) ann_lit list \<Rightarrow> 'a literal \<Rightarrow> bool option nres" where
-  \<open>valued' M L = nfoldli [0..<length M]
-  (\<lambda>v. is_None v)
-  (\<lambda>i v.
-    do {
-      if True (* atm_of (lit_of (op_list_get M i)) = atm_of L *)
-      then
-        if op_list_get M i = op_list_get M i
-        then do {RETURN (Some True)}
-        else do {RETURN (Some False)}
-      else do {RETURN (None)}
-    })
-  None\<close>
-
-definition test :: "('a, 'b) ann_lit list \<Rightarrow> nat \<Rightarrow> bool nres" where
-  \<open>test M i = do {ASSERT(i < length M); RETURN (op_list_get M i = op_list_get M i)}\<close>
-
-sepref_register \<open>valued\<close>
-
-term set_rel term map2
-
-type_synonym lit_refined = \<open>int\<close>
-
-
-record lit_prop = lvl :: nat cause :: nat
-
-type_synonym trail_refined = \<open>lit_refined list \<times> nat option list \<times> int list\<close>
-
-fun lit_of_refined :: \<open>int \<Rightarrow> nat literal\<close> where
-  \<open>lit_of_refined n = (if n < 0 then Neg (nat (-n)) else Pos (nat n))\<close>
-
-context
-  fixes N :: nat
-begin
-
-fun trail_of_refined :: "(nat, nat) ann_lit list \<Rightarrow> trail_refined \<Rightarrow> bool" where
-  \<open>trail_of_refined M (Ls, Ls', _) \<longleftrightarrow>
-    map2
-      (\<lambda>L n. if n = None then Decided (lit_of_refined L) else Propagated (lit_of_refined L) (the n))
-      (rev Ls) (rev Ls') =  M\<close>
-
-  term trail_rel
-definition trail_ref_rel :: "(trail_refined \<times> (nat, nat) ann_lits) set" where trail_rel_def_internal:
-  \<open>trail_ref_rel = {((lit_order, reasons, assignement), M). trail_of_refined M (lit_order, reasons, assignement) \<and>
-     length reasons = length lit_order(*  \<and>
-     (\<forall>L. lit_of_refined L \<in> lits_of_l M \<longrightarrow> sgn (assignement!(nat (abs L))) = sgn L) *)}\<close>
-
-lemmas trail_ref_rel_def[refine_rel_defs] = trail_rel_def_internal
-
-fun assign_lit :: \<open>(nat, nat) ann_lit \<Rightarrow> trail_refined \<Rightarrow> trail_refined\<close> where
-  \<open>assign_lit (Propagated (Pos L) C) (lit_order, reasons, assignement) =
-     (lit_order @ [(int L)], reasons @ [Some C], list_update assignement L (abs (assignement ! L)))\<close>
-|  \<open>assign_lit (Propagated (Neg L) C) (lit_order, reasons, assignement) =
-     (lit_order @ [-(int L)], reasons @ [Some C], list_update assignement L (-abs (assignement ! L)))\<close>
-|  \<open>assign_lit (Decided (Pos L)) (lit_order, reasons, assignement) =
-     (lit_order @ [(int L)], reasons @ [None], list_update assignement L (-abs (assignement ! L)))\<close>
-|  \<open>assign_lit (Decided (Neg L)) (lit_order, reasons, assignement) =
-     (lit_order @ [-(int L)], reasons @ [None], list_update assignement L (-abs (assignement ! L)))\<close>
-
-fun assign_Decided_lit :: \<open>int \<Rightarrow> trail_refined \<Rightarrow> trail_refined\<close> where
-   \<open>assign_Decided_lit L (lit_order, reasons, assignement) =
-     (lit_order @ [L], reasons @ [None], list_update assignement (nat (abs L)) (-abs (assignement ! nat (abs L))))\<close>
-
-definition ann_lit_rel where ann_lit_rel_def_internal:
-  "ann_lit_rel R \<equiv> {(l,l'). rel_ann_lit (\<lambda>x x'. (x,x')\<in>fst R) (\<lambda>x x'. (x,x')\<in>snd R) l l'}"
-
-abbreviation literal_rel :: "(nat literal \<times> nat literal) set" where
-"literal_rel \<equiv> Id::(nat literal \<times>_) set"
-
-definition nat_lit_int_assn :: "nat literal \<Rightarrow> int \<Rightarrow> assn" where
-  \<open>nat_lit_int_assn = pure {(L', L). L = lit_of_refined L'}\<close>
-
-sepref_decl_op Pos': "Pos :: nat \<Rightarrow> nat literal" ::  "nat_rel \<rightarrow> literal_rel" .
-
-lemma [def_pat_rules]:
-  "Pos \<equiv> op_Pos'"
-  by auto
-
-term id_assn
-
-definition literal_assn where
-"literal_assn \<equiv> hr_comp nat_assn {(L', L). L = lit_of_refined L'}"
-
-lemmas [safe_constraint_rules] = CN_FALSEI[of is_pure "literal_assn"]
-
-lemma [sepref_import_param]: \<open>(RETURN \<circ> Pos, RETURN o Pos) \<in> Id \<rightarrow> \<langle>Id\<rangle>nres_rel\<close>
-  by (auto simp: nres_rel_def)
-
-end
-
-context
-  notes [fcomp_norm_unfold] = literal_assn_def[symmetric]
-  notes [intro!] = hfrefI hn_refineI[THEN hn_refine_preI] frefI
-  notes [simp] = pure_def hn_ctxt_def invalid_assn_def
-begin
-  lemma int_Pos_refine[sepref_fr_rules]: \<open>(return o int, RETURN o op_Pos') \<in> nat_assn\<^sup>k \<rightarrow>\<^sub>a nat_lit_int_assn\<close>
-    unfolding nat_lit_int_assn_def by sep_auto
-  sepref_decl_impl trscp: int_Pos_refine .
-end
-term test
-
-definition test2 :: \<open>nat \<Rightarrow> nat literal nres\<close> where
-  \<open>test2 n = do {ASSERT (n > 0);  RETURN (Pos n)}\<close>
-term arl_length
-
-sepref_definition test' is test2 :: \<open>nat_assn\<^sup>k \<rightarrow>\<^sub>a nat_lit_int_assn\<close>
-  unfolding test2_def
-  apply sepref
-  done
-
-sepref_decl_intf nat_lit is "nat literal"
-
-(* lemma [sepref_import_param]: \<open>(RETURN \<circ> Pos, RETURN o Pos) \<in> Id \<rightarrow> \<langle>Id\<rangle>nres_rel\<close>
-  by (auto simp: nres_rel_def) *)
-
-
-definition nat_lits_trail_assn :: "(nat, nat) ann_lit list \<Rightarrow> trail_refined \<Rightarrow> assn" where
-  \<open>nat_lits_trail_assn = pure trail_ref_rel\<close>
-
-sepref_decl_op cons_Decided_lit': "(\<lambda>L M. Decided L # M) :: nat literal \<Rightarrow> (nat, nat) ann_lits \<Rightarrow> (nat, nat) ann_lits" ::
-   "(Id :: (nat literal \<times> _) set ) \<rightarrow> (Id :: ((nat, nat) ann_lits \<times> _) set) \<rightarrow>
-   (Id :: ((nat, nat) ann_lits \<times> _) set)"
-    .
-
-
-lemma assign_lit_cons_trail_ref_rel:
-  \<open>((aa, ab, b), ba) \<in> trail_ref_rel \<Longrightarrow> 0 < atm_of (lit_of a) \<Longrightarrow>
-  (assign_lit a (aa, ab, b), a # ba) \<in> trail_ref_rel\<close>
-  unfolding trail_ref_rel_def
-  apply (cases a; cases \<open>lit_of a\<close>)
-  by auto
-
-lemma assign_Decided_lit_cons_trail_ref_rel:
-  \<open>ai < 0 \<Longrightarrow>
-       ((a, aa, ba), b) \<in> trail_ref_rel \<Longrightarrow>
-       (ab, bb) \<Turnstile> emp \<Longrightarrow>
-       ((a @ [ai], aa @ [None], ba[nat (- ai) := - \<bar>ba ! nat (- ai)\<bar>]),
-        Decided (Neg (nat (- ai))) # b)
-       \<in> trail_ref_rel\<close>
-  \<open>0 < ai \<Longrightarrow>
-       ((a, aa, ba), b) \<in> trail_ref_rel \<Longrightarrow>
-       (ab, bb) \<Turnstile> emp \<Longrightarrow>
-       ((a @ [ai], aa @ [None], ba[nat ai := - \<bar>ba ! nat ai\<bar>]),
-        Decided (Pos (nat ai)) # b)
-       \<in> trail_ref_rel\<close>
-  unfolding trail_ref_rel_def
-  by auto
-
-context
-  notes [fcomp_norm_unfold] = array_assn_def[symmetric]
-  notes [intro!] = hfrefI hn_refineI[THEN hn_refine_preI]
-  notes [simp] = pure_def hn_ctxt_def is_array_def invalid_assn_def
-begin
-term \<open> (\<lambda>a b. nat_lit_int_assn b a)\<close>
-lemma assign_lit[sepref_fr_rules]:
-  \<open>(uncurry (return oo assign_Decided_lit), uncurry (RETURN oo op_cons_Decided_lit')) \<in>
-    [\<lambda>(L :: nat literal, M). atm_of L \<noteq> 0]\<^sub>a (\<lambda>a b. nat_lit_int_assn a b)\<^sup>k *\<^sub>a nat_lits_trail_assn\<^sup>d \<rightarrow> nat_lits_trail_assn\<close>
-  unfolding nat_lits_trail_assn_def
-  by sepref_to_hoare (sep_auto simp: nat_lit_int_assn_def assign_Decided_lit_cons_trail_ref_rel)
-
-thm HOL_list_prepend_hnr[sepref_fr_rules]
-
-lemmas [safe_constraint_rules] = CN_FALSEI[of is_pure "nat_lits_trail_assn"]
-sepref_decl_impl trscp2: assign_lit
-  apply auto
-  .
-
-end
-
-lemma [def_pat_rules]:
-  \<open>op # $ (Decided $ L) $ M \<equiv> op_cons_Decided_lit' $ L $ M\<close>
-  by auto
-thm def_pat_rules
-
-text \<open>We don't want to use the translation to \<^term>\<open>op_cons_lit'\<close> instead of
-  \<^term>\<open>op_list_prepend\<close>:\<close>
-declare Sepref_Id_Op.def_pat_rules(47)[def_pat_rules del]
-
-definition test3 :: \<open>nat literal \<Rightarrow> (nat, nat) ann_lits \<Rightarrow> (nat, nat) ann_lits nres\<close> where
-  \<open>test3 L M = do {ASSERT (atm_of L > 0);  RETURN (Decided L # M)}\<close>
-
-definition positive_lit_id where
-  \<open>positive_lit_id = pure {(L', L). L = L' \<and>  atm_of (lit_of L) > 0}\<close>
-
-sepref_definition test_42 is \<open>uncurry test3\<close> :: \<open>nat_lit_int_assn\<^sup>k *\<^sub>a nat_lits_trail_assn\<^sup>d \<rightarrow>\<^sub>a nat_lits_trail_assn\<close>
-  unfolding test3_def
-  apply sepref
-  done
-
-definition rand_nat :: \<open>nat \<Rightarrow> nat nres\<close> where
-  \<open>rand_nat n = SPEC (\<lambda>m. m \<le> n)\<close>
-sepref_register rand_nat
-(* sepref_decl_op rand_nat: rand_nat :: \<open>(Id :: (nat\<times>nat) set) \<rightarrow> (Id :: (nat \<times> nat) set)\<close>
-  apply (auto simp: rand_nat_def)
-  sorry
- *)
-
-
-definition rand_nat_stgy1 :: \<open>nat \<Rightarrow> nat\<close> where
-  \<open>rand_nat_stgy1 _ = 0\<close>
-
-context
-  notes [fcomp_norm_unfold] = array_assn_def[symmetric]
-  notes [intro!] = hfrefI hn_refineI[THEN hn_refine_preI]
-  notes [simp] = pure_def hn_ctxt_def is_array_def invalid_assn_def
-begin
-term \<open> (\<lambda>a b. nat_lit_int_assn b a)\<close>
-
-definition \<open>nat_pair \<equiv> pure {(m, n). True}\<close>
-
-lemma rand_nat_stgy[sepref_fr_rules]:
-  \<open>(return o rand_nat_stgy1, rand_nat) \<in> nat_assn\<^sup>k \<rightarrow>\<^sub>a nat_assn\<close>
-    apply (clarsimp intro!: nres_relI)
-  unfolding rand_nat_def rand_nat_stgy1_def nat_pair_def
-  by (sep_auto simp: rand_nat_def rand_nat_stgy1_def)
-
-end
-
-
-definition rand_rand :: \<open>nat \<Rightarrow> nat nres\<close> where
-  \<open>rand_rand n = do {n' \<leftarrow> rand_nat n; RETURN n'}\<close>
-
-sepref_definition rand_nat_stgy_test is rand_rand :: \<open>nat_assn\<^sup>k \<rightarrow>\<^sub>a nat_assn\<close>
-  unfolding rand_rand_def
-  apply sepref
-  done
-
+code_identifier
+  code_module DPLL_CDCL_W_Implementation \<rightharpoonup> (SML) CDCL_W_Level
+  
+prepare_code_thms backtrack_l'_impl_def
+export_code backtrack_l'_impl in SML
 end
